core/StateMachines.v
@@ -1,0 +1,277 @@
+Require Import Cheerios.Types.
+
+Require Import List.
+
+Import ListNotations.
+
+Module Type STATE_MACHINE.
+  Parameter run : forall {S A : Type},
+    (state_machine S A) -> S -> list byte -> fold_state S (A * list byte).
+
+  Parameter run_spec : forall {S A : Type}
+                              (f : state_machine S A)
+                              (s : S)
+                              (l : list byte),
+      run f s l =
+      match l with
+      | [] => More s
+      | b :: l => match f b s with
+                  | Done a => Done (a, l)
+                  | More s => run f s l
+                  | Error => Error
+                  end
+      end.
+
+  Parameter pair : forall {S1 A S2 B},
+      state_machine S1 A ->
+      state_machine S2 B -> state_machine (S1 * S2 + A * S2) (A * B).
+
+  Parameter run_pair_inr : forall S1 A S2 B
+                                  (a : state_machine S1 A) (b : state_machine S2 B)
+                                  x bytes s,
+      run (pair a b) (inr (x, s)) bytes =
+      match run b s bytes with
+      | Done (y, l)  => Done ((x, y), l)
+      | More s => More (inr (x, s))
+      | Error => Error
+      end.
+
+  Parameter run_pair_inl : forall S1 A S2 B
+                                  (a : state_machine S1 A) (b : state_machine S2 B)
+                                  bytes s1 s2,
+      run (pair a b) (inl (s1, s2)) bytes =
+      match run a s1 bytes with
+      | Done (x, l) => run (pair a b) (inr (x, s2)) l
+      | More s1 => More (inl (s1, s2))
+      | Error => Error
+      end.
+
+  Parameter sequence : forall {S1 A S2 B : Type},
+      state_machine S1 A -> state_machine S2 B -> state_machine (S1 * (A -> S2) + S2) B.
+
+  Parameter run_sequence_inr : forall S1 A S2 B
+                                      (a : state_machine S1 A)
+                                      (b : state_machine S2 B)
+                                      bytes s,
+      run (sequence a b) (inr s) bytes = match (run b s) bytes with
+                                         | Done (x, l) => Done (x, l)
+                                         | More s2 => More (inr s2)
+                                         | Error => Error
+                                         end.
+
+  Parameter run_sequence_inl : forall S1 A S2 B
+                                      (a : state_machine S1 A)
+                                      (b : state_machine S2 B)
+                                      bytes f s,
+      run (sequence a b) (inl (s, f)) bytes =
+      match run a s bytes with
+      | Done (x, bytes) => run (sequence a b) (inr (f x)) bytes
+      | More s1 => More (inl (s1, f))
+      | Error => Error
+      end.
+
+  
+
+  Parameter compose : forall {S1 A S2 B}, state_machine S1 A -> (state_machine S2 B) ->
+                                          (A -> fold_state S2 B) -> state_machine (S1 + S2) B.
+
+
+  Parameter map_sm : forall S A B, (A -> B) -> state_machine S A -> state_machine S B.
+
+End STATE_MACHINE.
+
+Module StateMachine : STATE_MACHINE.
+  Fixpoint run {S A}
+           (f : state_machine S A) (s : S) (l : list byte) : fold_state S (A * list byte) :=
+    match l with
+    | [] => More s
+    | b :: l => match f b s with
+                | Done a => Done (a, l)
+                | More s => run f s l
+                | Error => Error
+                end
+    end.
+
+  Lemma run_spec : forall {S A : Type}
+                          (f : state_machine S A)
+                          (s : S)
+                          (l : list byte),
+      run f s l =
+      match l with
+      | [] => More s
+      | b :: l => match f b s with
+                  | Done a => Done (a, l)
+                  | More s => run f s l
+                  | Error => Error
+                  end
+      end.
+  Proof.
+    now destruct l.
+  Qed.
+
+  Lemma run_append :
+    forall {S A : Type}  l1 l2 f (s : S),
+      @run S A f s (l1 ++ l2) =
+      match @run S A f s l1 with
+      | More s' => @run S A f s' l2
+      | Done (a, l1) => Done (a, l1 ++ l2)
+      | Error => Error
+      end.
+  Proof.
+    induction l1.
+    - intros.
+      reflexivity.
+    - intros.
+      simpl.
+      destruct (f a s);
+        try reflexivity.
+      rewrite IHl1.
+      reflexivity.
+  Qed.
+
+  
+  Definition pair {S1 A S2 B}
+             (a : state_machine S1 A)
+             (b : state_machine S2 B) : state_machine (S1 * S2 + A * S2) (A * B) :=
+    fun byte s =>
+      match s with
+      | inl (s1, s2) =>
+        match a byte s1 with
+        | Done x => More (inr (x, s2))
+        | More s1 => More (inl (s1, s2))
+        | Error => Error
+        end
+      | inr (x, s2) =>
+        match b byte s2 with
+        | Done b => Done (x, b)
+        | More s2 => More (inr (x, s2))
+        | Error => Error
+        end
+      end.
+
+  Lemma run_pair_inr : forall S1 A S2 B
+                              (a : state_machine S1 A) (b : state_machine S2 B)
+                              x bytes s,
+      run (pair a b) (inr (x, s)) bytes =
+      match run b s bytes with
+      | Done (y, l)  => Done ((x, y), l)
+      | More s => More (inr (x, s))
+      | Error => Error
+      end.
+  Proof.
+    intros until bytes.
+    induction bytes.
+    - reflexivity.
+    - intros s.
+      unfold run.
+      simpl.
+      destruct (b _ _);
+        auto.
+  Qed.
+
+  Lemma run_pair_inl : forall S1 A S2 B
+                              (a : state_machine S1 A) (b : state_machine S2 B)
+                              bytes s1 s2,
+      run (pair a b) (inl (s1, s2)) bytes =
+      match run a s1 bytes with
+      | Done (x, l) => run (pair a b) (inr (x, s2)) l
+      | More s1 => More (inl (s1, s2))
+      | Error => Error
+      end.
+  Proof.
+    intros until bytes.
+    induction bytes.
+    - reflexivity.
+    - intros.
+      simpl.
+      destruct a; auto.
+  Qed.
+
+
+  (* sequence takes two state machines and produces a state machine that will:
+     - run the first state machine
+     - apply a user-supplied mapping to the first machine's output to get the
+       initial state for the second machine, which will run from there *)
+  Definition sequence {S1 A S2 B}
+             (a : state_machine S1 A)
+             (b : state_machine S2 B) : state_machine (S1 * (A -> S2) + S2) B :=
+    fun byte s =>
+      match s with
+      | inl (s1, f) =>
+        match a byte s1 with
+        | Done x => More (inr (f x))
+        | More s1 => More (inl (s1, f))
+        | Error => Error
+        end
+      | inr s2 =>
+        match b byte s2 with
+        | Done b => Done b
+        | More s2 => More (inr s2)
+        | Error => Error
+        end
+      end.
+
+  Lemma run_sequence_inl : forall S1 A S2 B
+                                  (a : state_machine S1 A)
+                                  (b : state_machine S2 B)
+                                  bytes f s,
+      run (sequence a b) (inl (s, f)) bytes =
+      match run a s bytes with
+      | Done (x, bytes) => run (sequence a b) (inr (f x)) bytes
+      | More s1 => More (inl (s1, f))
+      | Error => Error
+      end.
+  Proof.
+    induction bytes.
+    - reflexivity.
+    - intros.
+      simpl.
+      destruct a;
+        auto.
+  Qed.
+
+  Lemma run_sequence_inr : forall S1 A S2 B
+                                  (a : state_machine S1 A)
+                                  (b : state_machine S2 B)
+                                  bytes s,
+      run (sequence a b) (inr s) bytes = match (run b s) bytes with
+                                         | Done (x, l) => Done (x, l)
+                                         | More s2 => More (inr s2)
+                                         | Error => Error
+                                         end.
+  Proof.
+    induction bytes; simpl; intros.
+    - reflexivity.
+    - destruct b; auto.
+  Qed.
+
+  Definition compose {S1 A S2 B}
+             (m1 : state_machine S1 A)
+             (m2 : state_machine S2 B)
+             (f : A -> fold_state S2 B) : state_machine (S1 + S2) B :=
+    fun b s =>
+      match s with
+      | inl s1 => match m1 b s1 with
+                  | Done a => match f a with
+                              | Done b => Done b
+                              | More s2 => More (inr s2)
+                              | Error => Error
+                              end
+                  | More s1 => More (inl s1)
+                  | Error => Error
+                  end
+      | inr s2 => match m2 b s2 with
+                  | Done b => Done b
+                  | More s2 => More (inr s2)
+                  | Error => Error
+                  end
+      end.
+
+  Definition map_sm {S A B} (f : A -> B) (m1: state_machine S A) : state_machine S B :=
+    fun b s =>
+      match m1 b s with
+      | Done a => Done (f a)
+      | More s => More s
+      | Error => Error
+      end.
+End StateMachine.
